Make file layout heap_lang consistent with auth.

heap_lang/heap.v
@@ -1,85 +1,80 @@
 From heap_lang Require Export derived.
 From program_logic Require Import ownership auth.
 Import uPred.
-
 (* TODO: The entire construction could be generalized to arbitrary languages that have
    a finmap as their state. Or maybe even beyond "as their state", i.e. arbitrary
    predicates over finmaps instead of just ownP. *)
-Section heap.
-  Definition heapRA := mapRA loc (exclRA (leibnizC val)).
-  Context {Σ : iFunctorG} (HeapI : gid) `{!InG heap_lang Σ HeapI (authRA heapRA)}.
-  Context (N : namespace).
 
+Definition heapRA := mapRA loc (exclRA (leibnizC val)).
+
+Class HeapInG Σ (i : gid) := heap_inG :> InG heap_lang Σ i (authRA heapRA).
+Instance heap_inG_auth `{HeapInG Σ i} : AuthInG heap_lang Σ i heapRA.
+Proof. split; apply _. Qed.
+
+Definition to_heap : state → heapRA := fmap Excl.
+Definition from_heap : heapRA → state := omap (maybe Excl).
+
+Lemma from_to_heap σ : from_heap (to_heap σ) = σ.
+Proof. apply map_eq=> l. rewrite lookup_omap lookup_fmap. by case (σ !! l). Qed.
+
+(* TODO: Do we want to expose heap ownership based on the state, or the heapRA?
+   The former does not expose the annoying "Excl", so for now I am going for
+   that. We should be able to derive the lemmas we want for this, too. *)
+Definition heap_own {Σ} (i : gid) `{HeapInG Σ i}
+  (γ : gname) (σ : state) : iPropG heap_lang Σ := auth_own i γ (to_heap σ).
+Definition heap_mapsto {Σ} (i : gid) `{HeapInG Σ i}
+  (γ : gname) (l : loc) (v : val) : iPropG heap_lang Σ := heap_own i γ {[ l ↦ v ]}.
+Definition heap_inv {Σ} (i : gid) `{HeapInG Σ i}
+  (h : heapRA) : iPropG heap_lang Σ := ownP (from_heap h).
+Definition heap_ctx {Σ} (i : gid) `{HeapInG Σ i}
+  (γ : gname) (N : namespace) : iPropG heap_lang Σ := auth_ctx i γ N (heap_inv i).
+
+Section heap.
+  Context {Σ : iFunctorG} (HeapI : gid) `{!HeapInG Σ HeapI}.
+  Implicit Types N : namespace.
   Implicit Types P : iPropG heap_lang Σ.
   Implicit Types σ : state.
   Implicit Types h g : heapRA.
   Implicit Types γ : gname.
 
-  Local Instance heap_auth : AuthInG heap_lang Σ HeapI heapRA.
-  Proof. split; intros; apply _. Qed.
-
-  Notation to_heap σ := (Excl <$> σ).
-  Definition from_heap : heapRA → state :=
-    omap (λ e, if e is Excl v then Some v else None).
-
-  Lemma from_to_heap σ : from_heap (to_heap σ) = σ.
-  Proof.
-    apply map_eq=>l. rewrite lookup_omap lookup_fmap.
-    (* FIXME RJ: To do case-analysis on σ !! l, I need to do this weird
-       "case _: ...". Neither destruct nor plain case work, I need the
-       one that generates an equality - but I do not need the equality.
-       This also happened in algebra/fin_maps.v. *)
-    by case _:(σ !! l)=>[v|] /=.
-  Qed.
-
-  (* TODO: Do we want to expose heap ownership based on the state, or the heapRA?
-     The former does not expose the annoying "Excl", so for now I am going for
-     that. We should be able to derive the lemmas we want for this, too. *)
-  Definition heap_own (γ : gname) (σ : state) : iPropG heap_lang Σ :=
-    auth_own HeapI γ (to_heap σ).
-  Definition heap_mapsto (γ : gname) (l : loc) (v : val) : iPropG heap_lang Σ :=
-    heap_own γ {[ l ↦ v ]}.
-  Definition heap_inv (h : heapRA) : iPropG heap_lang Σ :=
-    ownP (from_heap h).
-  Definition heap_ctx (γ : gname) : iPropG heap_lang Σ :=
-    auth_ctx HeapI γ N heap_inv.
-
-  Global Instance heap_inv_proper : Proper ((≡) ==> (≡)) heap_inv.
+  Global Instance heap_inv_proper : Proper ((≡) ==> (≡)) (heap_inv HeapI).
   Proof.
     move=>? ? EQ. rewrite /heap_inv /from_heap.
     (* TODO I guess we need some lemma about omap? *)
   Admitted. (* FIXME... I can't make progress otherwise... *)
 
   Lemma heap_own_op γ σ1 σ2 :
-    (heap_own γ σ1 ★ heap_own γ σ2)%I ≡ (■(σ1 ⊥ₘ σ2) ∧ heap_own γ (σ1 ∪ σ2))%I.
+    (heap_own HeapI γ σ1 ★ heap_own HeapI γ σ2)%I
+    ≡ (■ (σ1 ⊥ₘ σ2) ∧ heap_own HeapI γ (σ1 ∪ σ2))%I.
   Proof. (* TODO. *)
   Abort.
 
   Lemma heap_own_mapsto γ σ l v :
     (* TODO: Is this the best way to express "l ∉ dom σ"? *)
-    (heap_own γ σ ★ heap_mapsto γ l v)%I ≡ (■(σ !! l = None) ∧ heap_own γ (<[l:=v]>σ))%I.
+    (heap_own HeapI γ σ ★ heap_mapsto HeapI γ l v)%I
+    ≡ (■ (σ !! l = None) ∧ heap_own HeapI γ (<[l:=v]>σ))%I.
   Proof. (* TODO. *)
   Abort.
 
   (* TODO: Prove equivalence to a big sum. *)
 
-  Lemma heap_alloc σ :
-    ownP σ ⊑ pvs N N (∃ γ, heap_ctx γ ∧ heap_own γ σ).
+  Lemma heap_alloc N σ :
+    ownP σ ⊑ pvs N N (∃ γ, heap_ctx HeapI γ N ∧ heap_own HeapI γ σ).
   Proof.
     rewrite -{1}[σ]from_to_heap.
-    rewrite -(auth_alloc heap_inv N); first done.
+    rewrite -(auth_alloc _ N); first done.
     move=>n l. rewrite lookup_fmap. by case _:(σ !! l)=>[v|] /=.
   Qed.
 
-  Lemma wp_load_heap E γ σ l v P Q :
+  Lemma wp_load_heap N E γ σ l v P Q :
     nclose N ⊆ E →
     σ !! l = Some v →
-    P ⊑ heap_ctx γ →
-    P ⊑ (heap_own γ σ ★ ▷ (heap_own γ σ -★ Q v)) →
+    P ⊑ heap_ctx HeapI γ N →
+    P ⊑ (heap_own HeapI γ σ ★ ▷ (heap_own HeapI γ σ -★ Q v)) →
     P ⊑ wp E (Load (Loc l)) Q.
   Proof.
     rewrite /heap_ctx /heap_own. intros HN Hl Hctx HP.
-    eapply (auth_fsa heap_inv (wp_fsa (Load _) _) (λ _, True) id).
+    eapply (auth_fsa (heap_inv HeapI) (wp_fsa (Load _) _) (λ _, True) id).
     { eassumption. } { eassumption. }
     rewrite HP=>{HP Hctx HN}. apply sep_mono; first done.
     apply forall_intro=>hf. apply wand_intro_l. rewrite /heap_inv.
@@ -95,10 +90,10 @@ Section heap.
   { eexists. eauto. }
   Qed.
 
-  Lemma wp_load E γ l v P Q :
+  Lemma wp_load N E γ l v P Q :
     nclose N ⊆ E →
-    P ⊑ heap_ctx γ →
-    P ⊑ (heap_mapsto γ l v ★ ▷ (heap_mapsto γ l v -★ Q v)) →
+    P ⊑ heap_ctx HeapI γ N →
+    P ⊑ (heap_mapsto HeapI γ l v ★ ▷ (heap_mapsto HeapI γ l v -★ Q v)) →
     P ⊑ wp E (Load (Loc l)) Q.
   Proof.
     intros HN. rewrite /heap_mapsto. apply wp_load_heap; first done.
